Launchbury/ResourcedDenotational.thy
@@ -9,10 +9,10 @@ nominal_primrec
   CESem :: "exp \<Rightarrow> CEnv \<Rightarrow> CValue" ("\<N>\<lbrakk>_\<rbrakk>\<^bsub>_\<^esub>"  [60,60] 60)
 where
  "atom x \<sharp> \<rho> \<Longrightarrow>
-  \<N>\<lbrakk> Lam [x]. e \<rbrakk>\<^bsub>\<rho>\<^esub>  = (\<Lambda> (C \<cdot> _). CFn \<cdot> (\<Lambda> v r. (\<N>\<lbrakk> e \<rbrakk>\<^bsub>\<rho>(x f\<mapsto> v)\<^esub>) \<cdot> r))"
+  \<N>\<lbrakk> Lam [x]. e \<rbrakk>\<^bsub>\<rho>\<^esub>  = (\<Lambda> (C \<cdot> _). CFn \<cdot> (\<Lambda> v. \<N>\<lbrakk> e \<rbrakk>\<^bsub>\<rho>(x f\<mapsto> v)\<^esub>))"
   (* Do not use \<N>\<lbrakk> Var x \<rbrakk>\<^bsub>\<rho>\<^esub>  in the rule for App; it costs an additional
      resource and makes the adequacy proof difficult. *)
-| "\<N>\<lbrakk> App e x \<rbrakk>\<^bsub>\<rho>\<^esub>    = (\<Lambda> (C \<cdot> r).  ((\<N>\<lbrakk> e \<rbrakk>\<^bsub>\<rho>\<^esub>) \<cdot> r \<down>CFn (\<rho> f!\<^sub>\<bottom> x)) \<cdot> r)"  
+| "\<N>\<lbrakk> App e x \<rbrakk>\<^bsub>\<rho>\<^esub>    = (\<Lambda> (C \<cdot> r). ((\<N>\<lbrakk> e \<rbrakk>\<^bsub>\<rho>\<^esub>) \<cdot> r \<down>CFn (\<rho> f!\<^sub>\<bottom> x)) \<cdot> r)"
 | "\<N>\<lbrakk> Var x \<rbrakk>\<^bsub>\<rho>\<^esub>      = (\<Lambda> (C \<cdot> r). (\<rho> f!\<^sub>\<bottom> x) \<cdot> r)"
 | "set (bn as) \<sharp>* \<rho> \<Longrightarrow>
   \<N>\<lbrakk> Let as body \<rbrakk>\<^bsub>\<rho>\<^esub> = (\<Lambda> (C \<cdot> r). (\<N>\<lbrakk>body\<rbrakk>\<^bsub>has_ESem.HSem CESem (asToHeap as) \<rho>\<^esub>) \<cdot> r)"
